File no longer carries a data closure

File.v
@@ -1,29 +1,43 @@
 Require Import Coq.ZArith.ZArith.
 
 Require Import ByteData.
+Require Import FileSystems.
 
 Open Local Scope Z.
 
 Structure File := mkFile {
-  fileSystemId: Exc Z;
+  fileSystem: FileSystem;
   fileSize: Z;
   deleted: bool;
-  data: ByteData;
   lastAccess: Exc Z;
   lastModification: Exc Z;
   lastCreated: Exc Z;
   lastDeleted: Exc Z
 }.
 
+Definition isDeleted (file: File) := 
+  file.(deleted) = true.
 
+(*
 (* Treat negative values as counting back from the end of a file 
    (a la Python) *)
-Definition fetchByte (file: File) (offset: Z) := if (offset <? 0)
+Definition fetchByte (file: File) (offset: Z) (disk: Disk) := 
+  if (offset <? 0)
   then (file.(data) (file.(fileSize) + offset))
   else (file.(data) offset).
 
 (* Cleaner notation for file access. *)
 Notation "d @[ i ]" := (fetchByte d i) (at level 60).
 
-Definition isDeleted (file: File) := 
-  file.(deleted) = true.
+
+Definition fileEq (lhs rhs: @Fetch File) :=
+  match (lhs, rhs) with
+  | (Found lhs, Found rhs) =>
+      lhs.(fileSize) = rhs.(fileSize)
+      /\ lhs.(deleted) = rhs.(deleted)
+      /\ forall idx:Z, lhs @[ idx ] = rhs @[ idx ]
+  | (ErrorString lhs, ErrorString rhs) => lhs = rhs
+  | (MissingAt lhs, MissingAt rhs) => lhs = rhs
+  | _ => False
+  end.
+*)
