FileTypes.v
@@ -1,33 +1,35 @@
 Require Import Coq.ZArith.ZArith.
 
+Require Import ByteData.
 Require Import Fetch.
 Require Import File.
+Require Import FileData.
 
 Open Local Scope Z.
 
-Definition isJpeg (file: File) :=
-     file @[  0 ] = Found 255
-  /\ file @[  1 ] = Found 216 
-  /\ file @[ -2 ] = Found 255
-  /\ file @[ -1 ] = Found 217.
+Definition isJpeg (file: File) (disk: Disk) :=
+     file @[  0 | disk ] = Found 255
+  /\ file @[  1 | disk ] = Found 216 
+  /\ file @[ -2 | disk ] = Found 255
+  /\ file @[ -1 | disk ] = Found 217.
 
-Definition isGzip (file: File) :=
-     file @[  0 ] = Found 31
-  /\ file @[  1 ] = Found 139 
-  /\ file @[  2 ] = Found 8.
+Definition isGzip (file: File) (disk: Disk) :=
+     file @[  0 | disk ] = Found 31
+  /\ file @[  1 | disk ] = Found 139 
+  /\ file @[  2 | disk ] = Found 8.
 
-Definition isElf (file: File) :=
-     file @[  0 ] = Found 127
-  /\ file @[  1 ] = Found 69 
-  /\ file @[  2 ] = Found 76
-  /\ file @[  3 ] = Found 70.
+Definition isElf (file: File) (disk: Disk) :=
+     file @[  0 | disk ] = Found 127
+  /\ file @[  1 | disk ] = Found 69 
+  /\ file @[  2 | disk ] = Found 76
+  /\ file @[  3 | disk ] = Found 70.
 
 
-Lemma jpeg_is_not_gzip : forall (file: File),
-  (isJpeg file) -> ~ (isGzip file).
+Lemma jpeg_is_not_gzip : forall (file: File) (disk: Disk),
+  (isJpeg file disk) -> ~ (isGzip file disk).
 Proof.
   unfold isGzip, isJpeg.
-  intros file jpeg_asmpt.
+  intros file disk jpeg_asmpt.
   destruct jpeg_asmpt as [byte0_is_255]. rewrite byte0_is_255.
   unfold not. intros contra. destruct contra as [not_equal].
   discriminate not_equal.
