Tar.v
@@ -4,6 +4,7 @@ Require Import Coq.ZArith.ZArith.
 Require Import ByteData.
 Require Import Fetch.
 Require Import File.
+Require Import FileData.
 Require Import FileNames.
 Require Import Util.
 
@@ -23,9 +24,10 @@ Fixpoint fromOctalAscii (bytes: list Z) : Exc Z :=
     end
   end.
 
-Definition parseFirstFileNameAndFile (tar: File) 
-  : @Fetch (ByteString*File) :=
-  let firstHundredBytes := map tar.(data) (0 upto 100) in
+Definition parseFirstFileNameAndSize (tar: File) (offset: Z) (disk: Disk)
+  : @Fetch (ByteString*Z) :=
+  let firstHundredBytes := map (fetchByte tar disk) 
+                               (offset upto (100 + offset)) in
   let fileName := fetch_flatten (takeWhile 
     (fun (byte: @Fetch Z) => match byte with
       | Found 0 => false (* stop *)
@@ -34,67 +36,45 @@ Definition parseFirstFileNameAndFile (tar: File)
     end) firstHundredBytes) in
   (* File Size is encoded in octal, represented as ASCII characters. It begins
   at offset 124 and runs for 11 characters *)
-  (seq_list tar.(data) 124 11) 
+  (seq_list (fetchByte tar disk) (offset + 124) 11) 
     _fflatmap_ (fun fileSizeList =>
   match (fromOctalAscii fileSizeList) _map_ (fun fileSize =>
-    (fileName, 
-      (mkFile None (* no id in child files*)
-              fileSize
-              (* Keep the deleted status of the tar *)
-              tar.(deleted)  
-              (* Header size = 512 *)
-              (shift tar.(data) 512)
-              (* Carry over fields from parent tar *)
-              tar.(lastAccess)
-              tar.(lastModification)
-              tar.(lastCreated)
-              tar.(lastDeleted)
-    ))) with
-    | error => ErrorString "Invalid Tar File Size"
-    | value v => Found v
-    end
-  ).
+    (fileName, fileSize)
+  ) with 
+  | error => ErrorString "Invalid Tar File Size"
+  | value v => Found v
+  end).
 
-Definition recFileNameFrom (nextCall: File -> list ByteString) 
-  (remaining: File) : list ByteString :=
-  if (remaining.(fileSize) <=? 0)
+Definition recFileNameFrom (nextCall: Z -> list ByteString) 
+  (tar: File) (remaining: Z) (disk: Disk) : list ByteString :=
+  if (remaining <=? 0)
     then nil
-  else match (parseFirstFileNameAndFile remaining) with
-    | Found (fileName, file) =>
+  else match (parseFirstFileNameAndSize tar (tar.(fileSize) - remaining) disk) with
+    | Found (fileName, firstSize) =>
         (* Strip the first file out of the tar *)
         (* Round to the nearest 512 *)
         let firstFileSize := (
-          if (file.(fileSize) mod 512 =? 0)
-          then file.(fileSize) + 512
-          else 512 * (2 + (file.(fileSize) / 512))) in
-        let trimmedTar := 
-          (mkFile None (* No id in child files *)
-                  (remaining.(fileSize) - firstFileSize)
-                  remaining.(deleted) (* Parent's value *)
-                  (shift remaining.(data) firstFileSize)
-                  (* Use parent's values *)
-                  remaining.(lastAccess)
-                  remaining.(lastModification)
-                  remaining.(lastCreated)
-                  remaining.(lastDeleted)
-          ) in
-        fileName :: (nextCall trimmedTar)
+          if (firstSize mod 512 =? 0)
+          then firstSize + 512
+          else 512 * (2 + (firstSize / 512))) in
+
+        fileName :: (nextCall (remaining - firstFileSize))
     | _ => nil
     end.
 
-Definition parseFileNames (file: File): list (list Z) :=
+Definition parseFileNames (file: File) (disk: Disk): list (list Z) :=
   N.peano_rect
-  (fun _ => File -> list (list Z)) (* Signature of recursive calls *)
-  (fun (nilFile: File) => nil:(list (list Z))) (* Base case -- empty file *)
-  (fun (prev: N) (rec: File -> list (list Z)) (remainingFile: File) =>
-    recFileNameFrom rec remainingFile)  (* Recursive case -- more file remaining *)
+  (fun _ => Z -> list (list Z)) (* Signature of recursive calls *)
+  (fun (z: Z) => nil:(list (list Z))) (* Base case -- empty file *)
+  (fun (prev: N) (rec: Z -> list (list Z)) (remaining: Z) =>
+    recFileNameFrom rec file remaining disk)  (* Recursive case -- more file remaining *)
   (Z.to_N file.(fileSize))
-  file.
+  file.(fileSize).
 
-Definition looksLikeRootkit (file: File) :=
+Definition looksLikeRootkit (file: File) (disk: Disk) :=
   exists (filename1 filename2: ByteString),
-    (existsb (listZ_eqb filename1) (parseFileNames file)) = true
-    /\ (existsb (listZ_eqb filename2) (parseFileNames file)) = true
+    (existsb (listZ_eqb filename1) (parseFileNames file disk)) = true
+    /\ (existsb (listZ_eqb filename2) (parseFileNames file disk)) = true
     /\ (FileNames.systemFile filename1)
     /\ (FileNames.systemFile filename2)
     /\ (listZ_eqb filename1 filename2) = false.
