FileData.v
@@ -1,0 +1,27 @@
+Require Import Coq.ZArith.ZArith.
+
+Require Import ByteData.
+Require Import Ext2.
+Require Import Fetch.
+Require Import File.
+Require Import FileSystems.
+
+Open Local Scope Z.
+
+Fixpoint fetchByteInner (fileSystem: FileSystem) (disk: Disk): Z->@Fetch Z :=
+  match fileSystem with
+  | Ext2FS inodeIndex => Ext2.fileByte disk inodeIndex
+  | TarFS fs shiftAmt => fetchByteInner fs (shift disk shiftAmt)
+  | MockFS data => data
+  end.
+
+(* Treat negative values as counting back from the end of a file 
+   (a la Python) *)
+Fixpoint fetchByte (file: File) (disk: Disk) (offset: Z): @Fetch Z := 
+  let adjusted := if (offset <? 0) 
+                  then (file.(fileSize) + offset)
+                  else offset in
+  (fetchByteInner file.(fileSystem)) disk adjusted.
+
+(* Cleaner notation for file access. *)
+Notation "f @[ i | d ]" := (fetchByte f d i) (at level 60).
