FileSystems.v
@@ -1,6 +1,15 @@
 Require Import Coq.ZArith.ZArith.
 
 Require Import ByteData.
+
+Inductive FileSystem: Type :=
+  | Ext2FS: Z -> FileSystem
+  | TarFS: FileSystem -> Z -> FileSystem
+  | MockFS: ByteData -> FileSystem
+.
+
+(*
+Require Import ByteData.
 Require Import Ext2.
 Require Import Fetch.
 Require Import File.
@@ -12,17 +21,6 @@ Definition isOnDiskTry1 (file: File) (disk: Disk) :=
   (i >= 0 /\ i < file.(fileSize)) ->
     file @[ i ] = disk (start + i).
 
-Definition fileEq (lhs rhs: @Fetch File) :=
-  match (lhs, rhs) with
-  | (Found lhs, Found rhs) =>
-      lhs.(fileSize) = rhs.(fileSize)
-      /\ lhs.(deleted) = rhs.(deleted)
-      /\ forall idx:Z, lhs @[ idx ] = rhs @[ idx ]
-  | (ErrorString lhs, ErrorString rhs) => lhs = rhs
-  | (MissingAt lhs, MissingAt rhs) => lhs = rhs
-  | _ => False
-  end.
-
 Definition isOnDisk (file: File) (disk: Disk) :=
   (* Ext2 *)
   (exists (inodeIndex: Z),
@@ -30,3 +28,4 @@ Definition isOnDisk (file: File) (disk: Disk) :=
            (Found file))
   (* Disjunction with other file systems *)
 .
+*)
