Makefile
@@ -2,11 +2,12 @@ default:
 	coqc Fetch
 	coqc ByteData
 	coqc Util
+	coqc FileSystems
 	coqc File
 	coqc Ext2
 	coqc FileNames
+	coqc FileData
 	coqc FileTypes
-	coqc FileSystems
 	coqc Tar
 	coqc Timeline
 	coqc Ext2Lemmas
